## Page:
[[Discrete mathematical structures.pdf#page=76]]

## Topics:
#ProofTechniques;
#ProofByCases : [[2.3 Methods of proof#Proofs by cases]];
#Therefore : [[2.3 Methods of proof#Logically following]];
#Hypothesis : [[2.3 Methods of proof#Hypotheses]];
#Proving : [[2.3 Methods of proof#Proving]];
#RulesOfInference : [[2.3 Methods of proof#Rules of inference]];
#Equivalence : [[2.3 Methods of proof#Proving equivalence theorems]];
#ModusPonens : [[2.3 Methods of proof#The method of asserting]];
#IndirectProofMethod : [[2.3 Methods of proof#Indirect method]];
#ProofByContradiction : [[2.3 Methods of proof#Proof by contradiction]];
#StepsInProof : [[2.3 Methods of proof#Steps in proof]];

## Notes:

### Proofs by cases:
This proof type examines all possible truth values situations in a truth table.

### Logically following:
If an implication p $\to$ q is a tautology, where p and q may be compound statements, involving any number of propositional variables, we say that q **logically follows** from p. Suppose that an implication of the form:
$$(p_1 \space \land \space p_2 \space \land \space p_3 \space \land \space ... \space \land \space p_n) \to q$$
is a tautology. Then this implicaiton is true regardless of the truth values of any of its components. In this case, we say that q **logically follows** from $p_1, \space p_2, \space ..., \space p_n$. When q logically follows from $p_1, \space p_2, \space ..., \space p_n$, we write
$$
\displaylines{p_1 \\ p_2 \\ p_3 \\ . \\ . \\ . \\ p_n \\ \therefore \space \overline{q}}
$$
where the symbol $\therefore$ means therefore. This means that if we know that $p_1$ is true, $p_2$ is true, ..., and $p_n$ is true, then we know that q is true.

### Hypotheses:
Virtually, all mathematical theorems are composed of implications of the type
$$(p_1 \space \land \space p_2 \space \land \space p_3 \space \land \space ... \space \land \space p_n) \to q$$
The $p_i$'$s$ are called the **hypotheses** or **premises**, and q is called the **conclusion**.

### Proving:
To "**prove the theorem**" means to show that implication is a tautology. Note that we are not trying to show that q( the conclusion ) is true, but only that q will be true if all the $p_i$ are true. For this reason, mathematical proofs often begin with the statement "suppose that $p_1, \space p_2, \space ..., \space p_n$ are true" and conclude with the statement "therefore, q is true". The proof does not show that q is true, but simply shows that q has to be true if the $p_i$ are all true.

### Rules of inference:
Arguments bases on tautologies represents universally correct methods of reasoning. Their validity depends only on the form of the statements involved and not on the truth values of the variables that they contain. Such arguments are called **rules of inference**. The various steps in mathematical proof of a theorem must follow from the use of various rules of inference, and mathematical proof of a theorem must begin with the hypotheses, proceed through various steps, each justified by some rule of inference, and arrive at the conclusion.

### Example 1:
![[Pasted image 20230727140635.png]]

### Example 2:
![[Pasted image 20230727140738.png]]

### Example 3:
![[Pasted image 20230727141119.png]]

### Proving equivalence theorems:
Some mathematical theorems are equivalences, that is, they are of the form p $\leftrightarrow$ q. They are usually stated p if and only if q. By Example 3, the proof of such a theorem is logically equivalent with proving both p $\to$ q and q $\to$ p, and this is almost always the way in which equivalences are proved. We first assume that p is true, and show that q must then be true, next we assume that q is true and show that p must then be true.

### The method of asserting:
Or the **modus ponens**:
![[Pasted image 20230727141517.png]]

### Example 4:
![[Pasted image 20230727141730.png]]

### Example 5:
![[Draft_27-07-2023_14.19.13.excalidraw]]

### Indirect method:
An important proof technique called the indirect method follows from the tautology (p $\to$ q) $\leftrightarrow$ (~q $\to$ ~p). This states, as we previously mentioned, that an implication is equivalent to its contrapositive. Thus, to prove p $\to$ q indirectly, we assume that q is false (the statement ~q) and show that p is then false (the statement ~p).

### Example 6:
![[Pasted image 20230727151407.png]]
Solution: Let p: $n^2$ is odd and q: n is odd. We have to prove that p $\to$ q is true. Instead, we prove that ~q $\to$ ~p. Thus suppose that n is not odd so that n is even. Then n = 2k, where k is an integer. We have $n^2 = (2k)^2 = 4k^2 = 2(2k^2)$, so $n^2$ is even. We thus show that if n is even, then $n^2$ is even, which is the contrapositive of the given statement. Hence the given statement has been proved.

### Proof by contradiction:
This method is based on the tautology ((p $\to$ q) $\land$ (~q)) $\to$ (~p). Thus the rule of inference
![[Pasted image 20230727152339.png]]
is valid. Informally, this states that, if a statement p implies a false statement q, then p must be false. This is often applied to the case where q is an absurdity or contradiction, that is, a statement that is always false. An example is given by taking q as the contradiction r $\land$ ~r. Thus any statement that implies a contradiction must be false. In order to use proof by contradiction, suppose we wish to show that a statement q logically follows from statements $p_1, p_2, p_3, ..., p_n$. Assume that ~q is true (that is, q is false) as an extra hypothesis and that $p_1, p_2, p_3, ..., p_n$ are also true. If this enlarged hypothesis $p_1 \land p_2 \land p_3 \land ... \land p_n \land$~p implies a contradiction, then at least one of the statements $p_1, p_2, ..., p_n$ must be false. This means that if all the $p_i$'$s$ are true, then ~q must be false, so q must be true. Thus q follows from $p_1, p_2, ..., p_n$. This is **proof by contradiciton**.

### Example 7:
![[Pasted image 20230727153637.png]]
Solution: Assume $(p/q)^2$ = 2 for some integers p and q, which have no common factors. $(p/q)^2$ = 2 $\Leftrightarrow$ $p^2$ = 2$q^2$ => $p^2$ is even. This implies that p is even. Thus p = 2n for some integer n. We see that 2$q^2$ = $p^2$ = $(2n)^2$ = $4n^2$, so $q^2 = 2n^2$. Thus $q^2$ is even, and so q is even. We now have that both p and q are even and therefore have a common factor of 2. This is a contradiction to the assumption. Thus the assumption must be false. $\color{green}{\square}$

### Steps in proof:
In order to prove a theorem of the (typical) form ($p_1 \land p_2 \land ... \land p_n$) $\to$ q, we begin with the hypotheses $p_1, p_2, ..., p_n$ and show some other statement $r_1$ logically follows. Then, using $p_1, p_2, ..., p_n, r_1$, we show that some other statement $r_2$ logically follows. We continue this process, producing intermediate statemnts $r_1, r_2, ..., r_k$, called **steps in proof**, until we can finally show that the conclusion q logically follows from $p_1, p_2, ..., p_n, r_1, r_2, ..., r_k$. Each logical step must be justified by some valid proof technique based on the rules of inference that we have developed, or on some other rules that come from tautological implications we have not discussed. A t any stage, we can replace a statement that needs to be derived by its contrapositive statement or any other equivalent form.

### Example 8:
![[Pasted image 20230727165608.png]]
Let q: m = n, r: m = -n, and p: $n^2 = m^2$. We want to prove the theorem p $\leftrightarrow$ (q $\lor$ r). So we have to prove that s: p $\to$ (q $\lor$ r) and t: (q $\lor$ r) $\to$ p are true. Thus we asuume, that either q or r is true. If q is true, then $m^2$ = $n^2$, and if r is true, then $m^2$ = $(-n)^2$ = $n^2$, so either case p is true. We have therefore shown that the implication t is true. Now we must prove that s is true, that is, we assume p and try to prove either q or r. If p is true, then $n^2$ = $m^2$, so $m^2 - n^2 = 0$. But $m^2 - n^2 = (m - n)(m + n)$. If $r_1$ is the intermediate statement (m - n)(m + n) = 0, we have shownthat p $\to$ $r_1$ is true. We now show that $r_1$ $\to$ (q $\lor$ r) is true by showing that contrapositive ~(q $\lor$ r) $\to$ $\sim r_1$ is true. Now ~(q $\lor$ r) $\leftrightarrow$ (~q $\land$ ~r). Thus, if ~q: m $\neq$ n and ~r: m $\neq$ -n are true, then (m - n) $\neq$ 0 and (m+n) $\neq$ 0, so (m - n)(m + n) $\neq$ 0 and $r_1$ is false. We have therefore shown that $r_1$ $\to$ (q $\lor$ r) is true. Finally, from the truth of p $\to$ $r_1$ and $r_1$ $\to$ (q $\lor$ r), we can conclude that p $\to$ (q $\lor$ r) is true. $\color{green}{\square}$

### Final remark:
As a final remark, we remind the reader that many mathematical theorems actually mean the statement is true for all objects of a certain type. Sometimes this is not evident. Thus the theorem in Example 8 really states that, for all integers m and n, $m^2$ = $n^2$ if and only if m = n or m = -n. Similarly, the statemnt "If x and y are real numbers, and x $\neq$ y, then x $\lt$ y or y $\lt$ x" is a statement about all real numbers x and y. To prove such a theorem, we must make sure that the steps in the proof are valid for every real number. We could not assume, for example, that x is 2 or that y is $\pi$ or $\sqrt{3}$. This is why proofs often begin by selecting a generic element, denoted by a variable. On the other hand, we know from [[2.2 Conditional statements]], that the negation of a statemnt of the form $\forall$ x P(x) is $\exists$ x $\sim P(x)$, so we need only find a single example where the statement is false.

### Example 9:
![[Pasted image 20230728074938.png]]
Solution: To prove that $(x^2 = y^2) \leftrightarrow (x = y)$ we have to prove both implications $(x^2 = y^2) \to (x = y)$ and $(x^2 = y^2) \leftarrow (x = y)$. If we start with the first implication, and prove the contrapositive of it, we will observe that it is false, so it is the first implication as well, from where it results that the statement is false. The contrapositive of the first implication is (x $\neq$ y) $\to$ ($x^2 \neq y^2$). If it is true for all x and y, then the implication is true as well. But there are x, and y, for example x = 3 and y = -3, for which 3 $\neq$ -3, but $3^2 = (-3)^2$ . Using logical statements, the proof looks like this: We have to disprove that $\forall \space x \space \forall \space y \space (x \neq y) \to (x^2 \neq y^2)$, but if we find some x and y, for which $\exists \space x  \space \exists \space y \space (x \neq y) \land (x^2 = y^2)$, then the contrapositive of the first implication will be false, so will the statement too. For x = 3 and y = -3,
(3 $\neq$ -3) and ($3^2 = (-3)^2)$, so the negation of the contrapositive of the first implication is true, then the contrapositive is false, which means that the first implication is false as well, so the statement is disproved. $\color{green}{\square}$

### Proving and disproving:
In summary, if a statemnt claims that a property holds for all objects of a certain type, then, to prove it, we must use steps that are valid for all objects of that type and that do not make reference to any particular object. To disprove such a statement, we need only show one counterexample that is, one particular object or set of objects for which the claim fails.