## Page:
[[Discrete mathematical structures.pdf#page=82]]
## Topics:
#Proof ;
#MathematicalInduction : [[2.4 Mathematical induction#Proof by induction]];
## Notes:

### Proof by induction:
Here we discuss another proof technique. Suppose that the statement to be proved can be put in the form $\forall$ n $\ge$ n$_0$ P(n), where n$_0$ is some fixed integer. That is, suppose that we wish to show that P(n) is true for all $n \ge n_0.$ The following result shows how this can be done. Suppose that (a) P($n_0$) is true and (b) if P(k) is true for some k $\ge$ $n_0$, then P(k+1) must also be true. Then P(n) is true for all $n \ge n_0$. This result is called the **principle of mathematical induction**. Thus, to prove the truth of a statement $\forall \space n \ge n_0 \space P(n)$ using the principle of mathematical induction, we must begin by proving directly that the first proposition P($n_0$) is true. This is called the **basis step** of the induction and is generally very easy. Then, we must prove that P(k) $\to$ P(k + 1) is a tautology for any choice of $k \ge n_0$. Since the only case where an implication is false is if the **antecedent** is true and the **consequent** is false, this step is usually done by showing that, if P(k) were true, then P(k + 1) would also have to be true. Note that this is not the same as assuming that P(k) is true for some value k. This step is called the **induction step**, and some work will usually be required to show that the implication is always true.

### Example 1:
![[Pasted image 20230801231250.png]]
P(n) : 1+2+3+...+n = ( n(n + 1) ) / 2
Basis step: P(1) : 1 = ( 1(1 + 1) ) / 2 = 2 / 2 = 1 (true)
Induction step: Suppose that, for $k \ge 1$, P(k) is true, then P(k + 1) is also true:
P(k) : 1+2+3+...+k = ( k(k + 1) ) / 2 is true by assumption.
P(k + 1) : 1+2+3+...+k+k+1 = ( (k + 1)((k + 1) + 1) ) / 2 <=>
( k(k + 1) ) / 2 + (k + 1) = ( (k + 1)(k + 2) ) / 2 <=>
( k(k + 1) ) / 2 + ( 2(k + 1) )/2 = ( (k + 1)(k + 2) ) / 2 <=>
( k(k + 1) + 2(k + 1) ) / 2 = ( (k + 1)(k + 2) ) / 2 <=>
( (k + 1)(k + 2) ) / 2 = ( (k + 1)(k + 2) ) / 2 is also true, then P(n) is true for all n $\ge$ 1. $\color{green}{\square}$

### Example 2:
![[Pasted image 20230802095042.png]]
P(n) = $\overline{(\underset{i=1}{\overset{n}{\bigcup}} A_i)} = \underset{i=1}{\overset{n}{\bigcap}} \overline{A_i}$.
![[Draft_02-08-2023_10.14.14.excalidraw]]

### Example 3:
![[Pasted image 20230802112321.png]]
Let P(n) be the predicate that if A is any set with |A| = n $\ge$ 1, then A is countable.
Basis step: Here, $n_0 = 1$, so we let A be any set with one element, say A = {x}. In case x forms a sequence all by itself whose set is A, so P(1) is true.
Induction step: Suppose that if A is any set with k elements, then A is countable is true. Now, any set B with k+1 elements should be countable to. Pick any element x in B, since B - {x} is a set with k elements, the induction hypothesis P(k) tells us that there is a sequence $x_1, x_2, ..., x_k$ with B - {x} as its corresponding set. The sequence $x_1, x_2, ..., x_k, x$ has B as its corresponding set, so B is countable. Since B can be any set with k + 1 elements, P(k + 1) is true if P(k) is. Thus, by the principle of mathematical induction, P(n) is true for all n $\ge$ 1. $\color{green}{\square}$

### Example 4:
![[Pasted image 20230802113531.png]]
Let P(n) : n! $\ge$ $2^{n-2}$.
Basis step: Since $n_0$ = 1, P(1) : 1! $\ge$ $2^{1-1}$ <=>
1 $\ge$ $2^0$ <=> 1 $\ge$ 1 true.
Induction step:
Suppose that P(k) is true for all k $\ge$ 1. P(k) : k! $\ge$ $2^{k-1}$.
Prove P(k + 1) : (k + 1)! $\ge$ $2^{(k+1)-1}$ <=>
(k + 1)((k + 1) - 1)! $\ge$ $2^k$ <=>
(k + 1)(k)! $\ge$ $2^{k - 1}$ * 2 <=>
and because k + 1 is greater or equal to 2 for all k $\ge$ 1, then P(k + 1) is true if P(k) is true. Then P(n) is true for all n $\ge$ 1. $\color{green}{\square}$

### Example 5:
```
1. // Consider the following function given in pseudocode:
2. FUNCTION SQ(A)
	a. C = 0
	b. D = 0
	c. WHILE(D != A)
		1. C = C + A
		2. D = D + 1
	d. RETURN(C)
4. END OF FUNCTION SQ
```
The name of the function, SQ, suggests that it computes the square of A. Step 2.c.2. shows that A must be a positive integer if the looping is to end. A few trials with particular values of A will provide evidence that the function does carry out this task. However, suppose that we now want to prove that SQ always computes the square of the positive integer A, no matter how large A might be. We shall give a proof by mathematical induction. For each integer n $\ge$ 0, let $C_n$ and $D_n$ be the values of the variables C and D, respectively, after passing through the WHILE loop n times. In particular, $C_0$ and $D_0$ represent the values of the variables before looping starts. Let P(n) be the preciate $C_n$ = A x $D_n$. We shall prove by induction that $\forall \space n \ge 0 \space P(n)$ is true. Here $n_0$ = 0.
Basis step: P(0) is the statement $C_0 = A \space \text{x} \space D_0$ <=> 0 = A x 0 <=> 0 = 0 which is true.
Induction step: We must now use:
P(k) : $C_k = A \space \text{x} \space D_k$ to show that P(k + 1) : $C_{k+1} = A \space \text{x} \space D_{k+1}$ <=>
$C_k + A = A \space \text{x} \space (D_k + 1)$ <=>(using P(k) to replace $C_k$)<=>
$A \space \text{x} \space D_k + A = A \space \text{x} \space (D_k + 1)$ <=>
$A \space \text{x} \space (D_k + 1) = A \space \text{x} \space (D_k + 1)$ which is also true.
Then, by the principle of mathematical induction, P(n) is true for all n $\ge$ 0. $\color{green}{\square}$

### Example 6:
![[Pasted image 20230802124334.png]]
```
1. FUNCTION GCD(X, Y)
	a. WHILE(X != Y)
		1. IF (X > Y) THEN
			a. X = X - Y
		2. ELSE
			a. Y = Y - X
	b. RETURN(X)
2. END OF FUNCTION GCD
```
If X and Y are positive integers, then GCD returns GCD(X, Y). To prove this, let $X_n \space and \space Y_n$, be the values of X and Y after n $\ge$ 0 passes through the WHILE loop. We claim that P(n) : GCD($X_n, Y_n$) = GCD(X, Y) is true for all n $\ge$ 0, and we prove this by mathematical induction. Here $n_0$ is 0.
Basis step: $X_0$ = X, $Y_0$ = Y, since these are the values of the variables before looping begins; thus P(0) is the statement GCD($X_0, Y_0$) = GCD(X, Y), which is true.
Induction step: Now let us consider the left-hand side P(k + 1), that is, GCD($X_{k+1}, Y_{k+1}$). After the k + 1 pass through the loop either $X_{k+1}$ = $X_k$ and $Y_{k+1}$ = $Y_k - X_k$ or $X_{k+1} = X_k - Y_k$ and $Y_{k+1} = Y_k$. Then, if P(k) : GCD($X_k, Y_k$) = GCD(X, Y) is true, we have by [[1.4 Division in the integers]](Theorem 5), that GCD($X_{k+1}, Y_{k+1}$) = GCD($X_k, Y_k$) = GCD(X, Y). Thus, by the principle of mathematical induction, P(n) is true for all n $\ge$ 0. The exit condition for the loop is $X_n = Y_n$, and we have GCD($X_n, Y_n$) = $X_n$. Hence the function always returns the value GCD(X, Y). $\color{green}{\square}$